

## 答案

(1)  $\underline{7} + 2 = 9$

(2)  $2 + 7 = \underline{9}$

(3)  $5 - \underline{0} = 5$

(4)  $3 - 3 = \underline{0}$

(5)  $3 + 4 = \underline{7}$

(6)  $\underline{6} + 2 = 8$

(7)  $8 + 2 = \underline{10}$

(8)  $4 - 2 = \underline{2}$

(9)  $1 + 8 = \underline{9}$

(10)  $1 + 9 = \underline{10}$

(11)  $4 - \underline{1} = 3$

(12)  $3 - 1 = \underline{2}$

(13)  $5 - 3 = \underline{2}$

(14)  $9 + \underline{1} = 10$

(15)  $4 + \underline{4} = 8$

(16)  $8 - \underline{4} = 4$

(17)  $9 - \underline{7} = 2$

(18)  $10 - \underline{7} = 3$

(19)  $6 + \underline{3} = 9$

(20)  $5 - 2 = \underline{3}$

(21)  $2 - 1 = \underline{1}$

(22)  $\underline{8} - 7 = 1$

(23)  $7 - \underline{1} = 6$

(24)  $8 + \underline{1} = 9$

(25)  $7 - \underline{6} = 1$

(26)  $\underline{5} + 2 = 7$

(27)  $3 + \underline{6} = 9$

(28)  $2 + \underline{1} = 3$

(29)  $7 + 3 = \underline{10}$

(30)  $2 + 8 = \underline{10}$

# 答案

(1)  $2 - 1 = \underline{1}$

(2)  $\underline{1} + 8 = 9$

(3)  $9 - 0 = \underline{9}$

(4)  $0 + \underline{1} = 1$

(5)  $\underline{9} + 1 = 10$

(6)  $6 - 1 = \underline{5}$

(7)  $1 + 9 = \underline{10}$

(8)  $7 + \underline{3} = 10$

(9)  $9 - \underline{7} = 2$

(10)  $3 - 1 = \underline{2}$

(11)  $\underline{9} - 1 = 8$

(12)  $8 + \underline{2} = 10$

(13)  $5 - \underline{4} = 1$

(14)  $\underline{10} - 1 = 9$

(15)  $10 - 9 = \underline{1}$

(16)  $4 - 3 = \underline{1}$

(17)  $\underline{3} + 4 = 7$

(18)  $6 + \underline{3} = 9$

(19)  $2 + \underline{7} = 9$

(20)  $6 - 2 = \underline{4}$

(21)  $2 + 3 = \underline{5}$

(22)  $\underline{4} + 2 = 6$

(23)  $6 + \underline{4} = 10$

(24)  $\underline{7} + 1 = 8$

(25)  $\underline{5} + 4 = 9$

(26)  $\underline{3} + 6 = 9$

(27)  $2 + 1 = \underline{3}$

(28)  $8 + 1 = \underline{9}$

(29)  $4 + \underline{4} = 8$

(30)  $5 + 1 = \underline{6}$

## 答案

(1)  $\underline{5} + 3 = 8$

(2)  $\underline{0} + 1 = 1$

(3)  $8 + \underline{0} = 8$

(4)  $7 + \underline{3} = 10$

(5)  $7 - \underline{3} = 4$

(6)  $\underline{7} + 1 = 8$

(7)  $8 - \underline{6} = 2$

(8)  $6 + \underline{4} = 10$

(9)  $1 + 7 = \underline{8}$

(10)  $2 + 7 = \underline{9}$

(11)  $8 + \underline{2} = 10$

(12)  $10 - 7 = \underline{3}$

(13)  $4 + \underline{1} = 5$

(14)  $8 - 1 = \underline{7}$

(15)  $\underline{5} + 1 = 6$

(16)  $5 - \underline{1} = 4$

(17)  $6 + \underline{2} = 8$

(18)  $6 - 1 = \underline{5}$

(19)  $3 + \underline{2} = 5$

(20)  $\underline{9} + 1 = 10$

(21)  $\underline{4} + 5 = 9$

(22)  $1 + 1 = \underline{2}$

(23)  $2 + \underline{5} = 7$

(24)  $4 + \underline{2} = 6$

(25)  $10 - 2 = \underline{8}$

(26)  $9 - \underline{6} = 3$

(27)  $5 + \underline{4} = 9$

(28)  $10 - \underline{5} = 5$

(29)  $3 + \underline{7} = 10$

(30)  $\underline{9} - 4 = 5$

## 答案

(1)  $9 - \underline{5} = 4$

(2)  $2 + \underline{0} = 2$

(3)  $9 - \underline{1} = 8$

(4)  $6 + 1 = \underline{7}$

(5)  $\underline{6} - 1 = 5$

(6)  $\underline{0} + 1 = 1$

(7)  $\underline{4} - 2 = 2$

(8)  $\underline{7} - 2 = 5$

(9)  $\underline{1} + 9 = 10$

(10)  $9 + 1 = \underline{10}$

(11)  $8 - 2 = \underline{6}$

(12)  $3 - 1 = \underline{2}$

(13)  $5 + 5 = \underline{10}$

(14)  $7 - \underline{3} = 4$

(15)  $3 + \underline{7} = 10$

(16)  $8 - \underline{6} = 2$

(17)  $1 + 6 = \underline{7}$

(18)  $\underline{8} - 5 = 3$

(19)  $6 + 2 = \underline{8}$

(20)  $\underline{5} + 2 = 7$

(21)  $\underline{8} - 4 = 4$

(22)  $8 + 1 = \underline{9}$

(23)  $\underline{2} + 3 = 5$

(24)  $2 + \underline{7} = 9$

(25)  $9 - 4 = \underline{5}$

(26)  $\underline{2} + 1 = 3$

(27)  $7 + \underline{1} = 8$

(28)  $\underline{6} - 4 = 2$

(29)  $\underline{1} + 1 = 2$

(30)  $9 - 7 = \underline{2}$

## 答案

(1)  $6 + 3 = \underline{9}$

(2)  $3 + \underline{7} = 10$

(3)  $\underline{10} - 2 = 8$

(4)  $\underline{5} - 0 = 5$

(5)  $\underline{0} - 0 = 0$

(6)  $6 - \underline{3} = 3$

(7)  $7 - 2 = \underline{5}$

(8)  $\underline{10} - 5 = 5$

(9)  $3 + 4 = \underline{7}$

(10)  $3 - 2 = \underline{1}$

(11)  $\underline{8} - 2 = 6$

(12)  $9 - 5 = \underline{4}$

(13)  $1 + \underline{1} = 2$

(14)  $3 + \underline{5} = 8$

(15)  $7 - 3 = \underline{4}$

(16)  $1 + \underline{4} = 5$

(17)  $2 + \underline{7} = 9$

(18)  $\underline{6} - 1 = 5$

(19)  $\underline{5} + 2 = 7$

(20)  $4 + \underline{3} = 7$

(21)  $8 + 1 = \underline{9}$

(22)  $\underline{9} - 7 = 2$

(23)  $7 + \underline{3} = 10$

(24)  $6 + 4 = \underline{10}$

(25)  $8 - \underline{6} = 2$

(26)  $1 + \underline{9} = 10$

(27)  $2 - \underline{1} = 1$

(28)  $6 - 2 = \underline{4}$

(29)  $\underline{9} - 6 = 3$

(30)  $\underline{6} + 1 = 7$

## 答案

(1)  $8 - \underline{7} = 1$

(2)  $2 + \underline{8} = 10$

(3)  $1 + \underline{7} = 8$

(4)  $1 + 8 = \underline{9}$

(5)  $9 + \underline{1} = 10$

(6)  $9 + 0 = \underline{9}$

(7)  $\underline{0} + 0 = 0$

(8)  $7 - 3 = \underline{4}$

(9)  $\underline{6} - 4 = 2$

(10)  $5 - 1 = \underline{4}$

(11)  $\underline{3} + 3 = 6$

(12)  $6 - \underline{5} = 1$

(13)  $\underline{3} + 1 = 4$

(14)  $\underline{7} + 3 = 10$

(15)  $7 + 1 = \underline{8}$

(16)  $\underline{6} + 3 = 9$

(17)  $\underline{6} - 1 = 5$

(18)  $\underline{9} - 4 = 5$

(19)  $2 + 6 = \underline{8}$

(20)  $\underline{4} - 3 = 1$

(21)  $1 + 3 = \underline{4}$

(22)  $\underline{9} - 7 = 2$

(23)  $9 - \underline{2} = 7$

(24)  $7 - \underline{1} = 6$

(25)  $\underline{1} + 1 = 2$

(26)  $\underline{1} + 2 = 3$

(27)  $8 - \underline{1} = 7$

(28)  $\underline{6} - 3 = 3$

(29)  $\underline{8} - 2 = 6$

(30)  $2 - \underline{1} = 1$

# 答案

(1)  $4 - 4 = \underline{0}$

(2)  $\underline{2} - 1 = 1$

(3)  $7 - 4 = \underline{3}$

(4)  $9 - 3 = \underline{6}$

(5)  $10 + \underline{0} = 10$

(6)  $\underline{10} - 6 = 4$

(7)  $1 + \underline{6} = 7$

(8)  $\underline{9} - 8 = 1$

(9)  $6 + \underline{4} = 10$

(10)  $7 - 6 = \underline{1}$

(11)  $5 - 2 = \underline{3}$

(12)  $\underline{10} - 4 = 6$

(13)  $3 - \underline{2} = 1$

(14)  $\underline{6} + 3 = 9$

(15)  $\underline{3} + 6 = 9$

(16)  $2 + 1 = \underline{3}$

(17)  $5 - 4 = \underline{1}$

(18)  $8 + \underline{1} = 9$

(19)  $5 + \underline{2} = 7$

(20)  $\underline{7} - 3 = 4$

(21)  $\underline{8} - 5 = 3$

(22)  $3 + \underline{1} = 4$

(23)  $\underline{10} - 1 = 9$

(24)  $7 - \underline{5} = 2$

(25)  $4 + 2 = \underline{6}$

(26)  $2 + \underline{8} = 10$

(27)  $6 + 1 = \underline{7}$

(28)  $\underline{9} - 2 = 7$

(29)  $8 - \underline{3} = 5$

(30)  $5 + \underline{1} = 6$

## 答案

(1)  $4 - 1 = \underline{3}$

(2)  $\underline{10} + 0 = 10$

(3)  $2 + 1 = \underline{3}$

(4)  $4 + \underline{0} = 4$

(5)  $1 + \underline{4} = 5$

(6)  $2 - \underline{1} = 1$

(7)  $7 + 3 = \underline{10}$

(8)  $6 - \underline{5} = 1$

(9)  $5 + 4 = \underline{9}$

(10)  $7 - \underline{2} = 5$

(11)  $8 - \underline{2} = 6$

(12)  $2 + \underline{8} = 10$

(13)  $5 - \underline{3} = 2$

(14)  $6 - 1 = \underline{5}$

(15)  $8 - 3 = \underline{5}$

(16)  $\underline{3} + 5 = 8$

(17)  $6 + \underline{3} = 9$

(18)  $5 - 1 = \underline{4}$

(19)  $7 + 1 = \underline{8}$

(20)  $1 + 6 = \underline{7}$

(21)  $7 + 2 = \underline{9}$

(22)  $\underline{5} + 2 = 7$

(23)  $3 - \underline{1} = 2$

(24)  $6 + 4 = \underline{10}$

(25)  $2 + \underline{4} = 6$

(26)  $4 + 3 = \underline{7}$

(27)  $5 + 1 = \underline{6}$

(28)  $\underline{7} - 1 = 6$

(29)  $5 + \underline{3} = 8$

(30)  $\underline{8} + 2 = 10$



## 答案

(1)  $9 + \underline{0} = 9$

(2)  $4 - 0 = \underline{4}$

(3)  $4 - 3 = \underline{1}$

(4)  $3 - \underline{2} = 1$

(5)  $2 + 8 = \underline{10}$

(6)  $1 + \underline{9} = 10$

(7)  $\underline{1} + 4 = 5$

(8)  $6 - \underline{4} = 2$

(9)  $8 - \underline{3} = 5$

(10)  $9 - \underline{3} = 6$

(11)  $\underline{8} - 4 = 4$

(12)  $10 - 2 = \underline{8}$

(13)  $7 - \underline{4} = 3$

(14)  $6 - 3 = \underline{3}$

(15)  $4 + \underline{3} = 7$

(16)  $\underline{7} + 3 = 10$

(17)  $7 + 2 = \underline{9}$

(18)  $5 + 5 = \underline{10}$

(19)  $8 - \underline{5} = 3$

(20)  $3 + 4 = \underline{7}$

(21)  $\underline{4} - 2 = 2$

(22)  $\underline{8} + 2 = 10$

(23)  $\underline{7} - 6 = 1$

(24)  $\underline{7} - 5 = 2$

(25)  $2 + \underline{3} = 5$

(26)  $7 - 2 = \underline{5}$

(27)  $8 - \underline{6} = 2$

(28)  $\underline{7} + 1 = 8$

(29)  $\underline{2} + 2 = 4$

(30)  $9 + \underline{1} = 10$

## 答案

(1)  $0 + 8 = \underline{8}$

(2)  $\underline{2} + 3 = 5$

(3)  $10 + 0 = \underline{10}$

(4)  $5 - \underline{2} = 3$

(5)  $\underline{5} - 1 = 4$

(6)  $7 - 5 = \underline{2}$

(7)  $\underline{6} - 4 = 2$

(8)  $8 + \underline{2} = 10$

(9)  $3 + \underline{4} = 7$

(10)  $\underline{5} - 3 = 2$

(11)  $\underline{7} - 2 = 5$

(12)  $\underline{6} - 3 = 3$

(13)  $7 + \underline{3} = 10$

(14)  $\underline{9} + 1 = 10$

(15)  $\underline{6} - 2 = 4$

(16)  $9 - \underline{7} = 2$

(17)  $\underline{6} + 3 = 9$

(18)  $9 - 6 = \underline{3}$

(19)  $\underline{2} + 4 = 6$

(20)  $8 - \underline{5} = 3$

(21)  $\underline{6} + 4 = 10$

(22)  $\underline{2} + 7 = 9$

(23)  $9 - 2 = \underline{7}$

(24)  $\underline{7} - 6 = 1$

(25)  $1 + 1 = \underline{2}$

(26)  $\underline{8} - 2 = 6$

(27)  $6 - \underline{1} = 5$

(28)  $\underline{5} + 4 = 9$

(29)  $6 + \underline{2} = 8$

(30)  $\underline{6} - 5 = 1$